src/HOL/MicroJava/J/WellType.thy
@@ -21,16 +21,17 @@ methods of class Object to be called upon references of interface type.
 \end{itemize}
 \end{description}
 *}
-types	lenv (* local variables, including method parameters and This *)
-	= "vname \<leadsto> ty"
-        'c env
-	= "'c prog \<times> lenv"
+
+text "local variables, including method parameters and This:"
+types 
+  lenv   = "vname \<leadsto> ty"
+  'c env = "'c prog \<times> lenv"
 
 syntax
   prg    :: "'c env => 'c prog"
   localT :: "'c env => (vname \<leadsto> ty)"
 
-translations	
+translations  
   "prg"    => "fst"
   "localT" => "snd"
 
@@ -42,15 +43,15 @@ consts
 
 defs
   more_spec_def: "more_spec G == \<lambda>((d,h),pTs). \<lambda>((d',h'),pTs'). G\<turnstile>d\<preceq>d' \<and>
-		                            list_all2 (\<lambda>T T'. G\<turnstile>T\<preceq>T') pTs pTs'"
+                                list_all2 (\<lambda>T T'. G\<turnstile>T\<preceq>T') pTs pTs'"
   
-  (* applicable methods, cf. 15.11.2.1 *)
+  -- "applicable methods, cf. 15.11.2.1"
   appl_methds_def: "appl_methds G C == \<lambda>(mn, pTs).
-		                 {((Class md,rT),pTs') |md rT mb pTs'.
-		                  method (G,C)  (mn, pTs') = Some (md,rT,mb) \<and>
-		                  list_all2 (\<lambda>T T'. G\<turnstile>T\<preceq>T') pTs pTs'}"
+                     {((Class md,rT),pTs') |md rT mb pTs'.
+                      method (G,C)  (mn, pTs') = Some (md,rT,mb) \<and>
+                      list_all2 (\<lambda>T T'. G\<turnstile>T\<preceq>T') pTs pTs'}"
 
-  (* maximally specific methods, cf. 15.11.2.2 *)
+  -- "maximally specific methods, cf. 15.11.2.2"
   max_spec_def: "max_spec G C sig == {m. m \<in>appl_methds G C sig \<and> 
                                        (\<forall>m'\<in>appl_methds G C sig.
                                          more_spec G m' m --> m' = m)}"
@@ -77,13 +78,14 @@ consts
   typeof :: "(loc => ty option) => val => ty option"
 
 primrec
-	"typeof dt  Unit    = Some (PrimT Void)"
-	"typeof dt  Null    = Some NT"
-	"typeof dt (Bool b) = Some (PrimT Boolean)"
-	"typeof dt (Intg i) = Some (PrimT Integer)"
-	"typeof dt (Addr a) = dt a"
+  "typeof dt  Unit    = Some (PrimT Void)"
+  "typeof dt  Null    = Some NT"
+  "typeof dt (Bool b) = Some (PrimT Boolean)"
+  "typeof dt (Intg i) = Some (PrimT Integer)"
+  "typeof dt (Addr a) = dt a"
 
-lemma is_type_typeof [rule_format (no_asm), simp]: "(\<forall>a. v \<noteq> Addr a) --> (\<exists>T. typeof t v = Some T \<and> is_type G T)"
+lemma is_type_typeof [rule_format (no_asm), simp]: 
+  "(\<forall>a. v \<noteq> Addr a) --> (\<exists>T. typeof t v = Some T \<and> is_type G T)"
 apply (rule val.induct)
 apply     auto
 done
@@ -95,9 +97,9 @@ apply     auto
 done
 
 types
-	java_mb = "vname list \<times> (vname \<times> ty) list \<times> stmt \<times> expr"
-(* method body with parameter names, local variables, block, result expression.
-   local variables might include This, which is hidden anyway *)
+  java_mb = "vname list \<times> (vname \<times> ty) list \<times> stmt \<times> expr"
+-- "method body with parameter names, local variables, block, result expression."
+-- "local variables might include This, which is hidden anyway"
 
 consts
   ty_expr :: "java_mb env => (expr      \<times> ty     ) set"
@@ -116,30 +118,27 @@ syntax
 
 
 translations
-	"E\<turnstile>e :: T" == "(e,T) \<in> ty_expr  E"
-	"E\<turnstile>e[::]T" == "(e,T) \<in> ty_exprs E"
-	"E\<turnstile>c \<surd>"    == "c     \<in> wt_stmt  E"
+  "E\<turnstile>e :: T" == "(e,T) \<in> ty_expr  E"
+  "E\<turnstile>e[::]T" == "(e,T) \<in> ty_exprs E"
+  "E\<turnstile>c \<surd>"    == "c     \<in> wt_stmt  E"
   
 inductive "ty_expr E" "ty_exprs E" "wt_stmt E" intros
+  
+  NewC: "[| is_class (prg E) C |] ==>
+         E\<turnstile>NewC C::Class C"  -- "cf. 15.8"
 
-(* well-typed expressions *)
-
-  (* cf. 15.8 *)
-  NewC:	"[| is_class (prg E) C |] ==>
-         E\<turnstile>NewC C::Class C"
-
-  (* cf. 15.15 *)
-  Cast:	"[| E\<turnstile>e::Class C; is_class (prg E) D;
+  -- "cf. 15.15"
+  Cast: "[| E\<turnstile>e::Class C; is_class (prg E) D;
             prg E\<turnstile>C\<preceq>? D |] ==>
          E\<turnstile>Cast D e::Class D"
 
-  (* cf. 15.7.1 *)
-  Lit:	  "[| typeof (\<lambda>v. None) x = Some T |] ==>
+  -- "cf. 15.7.1"
+  Lit:    "[| typeof (\<lambda>v. None) x = Some T |] ==>
          E\<turnstile>Lit x::T"
 
   
-  (* cf. 15.13.1 *)
-  LAcc:	"[| localT E v = Some T; is_type (prg E) T |] ==>
+  -- "cf. 15.13.1"
+  LAcc: "[| localT E v = Some T; is_type (prg E) T |] ==>
          E\<turnstile>LAcc v::T"
 
   BinOp:"[| E\<turnstile>e1::T;
@@ -148,42 +147,42 @@ inductive "ty_expr E" "ty_exprs E" "wt_stmt E" intros
                         else T' = T \<and> T = PrimT Integer|] ==>
             E\<turnstile>BinOp bop e1 e2::T'"
 
-  (* cf. 15.25, 15.25.1 *)
+  -- "cf. 15.25, 15.25.1"
   LAss: "[| v ~= This;
             E\<turnstile>LAcc v::T;
-	    E\<turnstile>e::T';
+      E\<turnstile>e::T';
             prg E\<turnstile>T'\<preceq>T |] ==>
          E\<turnstile>v::=e::T'"
 
-  (* cf. 15.10.1 *)
+  -- "cf. 15.10.1"
   FAcc: "[| E\<turnstile>a::Class C; 
             field (prg E,C) fn = Some (fd,fT) |] ==>
             E\<turnstile>{fd}a..fn::fT"
 
-  (* cf. 15.25, 15.25.1 *)
+  -- "cf. 15.25, 15.25.1"
   FAss: "[| E\<turnstile>{fd}a..fn::T;
             E\<turnstile>v        ::T';
             prg E\<turnstile>T'\<preceq>T |] ==>
          E\<turnstile>{fd}a..fn:=v::T'"
 
 
-  (* cf. 15.11.1, 15.11.2, 15.11.3 *)
+  -- "cf. 15.11.1, 15.11.2, 15.11.3"
   Call: "[| E\<turnstile>a::Class C;
             E\<turnstile>ps[::]pTs;
             max_spec (prg E) C (mn, pTs) = {((md,rT),pTs')} |] ==>
          E\<turnstile>{C}a..mn({pTs'}ps)::rT"
 
-(* well-typed expression lists *)
+-- "well-typed expression lists"
 
-  (* cf. 15.11.??? *)
+  -- "cf. 15.11.???"
   Nil: "E\<turnstile>[][::][]"
 
-  (* cf. 15.11.??? *)
+  -- "cf. 15.11.???"
   Cons:"[| E\<turnstile>e::T;
            E\<turnstile>es[::]Ts |] ==>
         E\<turnstile>e#es[::]T#Ts"
 
-(* well-typed statements *)
+-- "well-typed statements"
 
   Skip:"E\<turnstile>Skip\<surd>"
 
@@ -194,13 +193,13 @@ inductive "ty_expr E" "ty_exprs E" "wt_stmt E" intros
            E\<turnstile>s2\<surd> |] ==>
         E\<turnstile>s1;; s2\<surd>"
 
-  (* cf. 14.8 *)
+  -- "cf. 14.8"
   Cond:"[| E\<turnstile>e::PrimT Boolean;
            E\<turnstile>s1\<surd>;
            E\<turnstile>s2\<surd> |] ==>
          E\<turnstile>If(e) s1 Else s2\<surd>"
 
-  (* cf. 14.10 *)
+  -- "cf. 14.10"
   Loop:"[| E\<turnstile>e::PrimT Boolean;
            E\<turnstile>s\<surd> |] ==>
         E\<turnstile>While(e) s\<surd>"
@@ -209,14 +208,14 @@ constdefs
 
  wf_java_mdecl :: "java_mb prog => cname => java_mb mdecl => bool"
 "wf_java_mdecl G C == \<lambda>((mn,pTs),rT,(pns,lvars,blk,res)).
-	length pTs = length pns \<and>
-	nodups pns \<and>
-	unique lvars \<and>
+  length pTs = length pns \<and>
+  nodups pns \<and>
+  unique lvars \<and>
         This \<notin> set pns \<and> This \<notin> set (map fst lvars) \<and> 
-	(\<forall>pn\<in>set pns. map_of lvars pn = None) \<and>
-	(\<forall>(vn,T)\<in>set lvars. is_type G T) &
-	(let E = (G,map_of lvars(pns[\<mapsto>]pTs)(This\<mapsto>Class C)) in
-	 E\<turnstile>blk\<surd> \<and> (\<exists>T. E\<turnstile>res::T \<and> G\<turnstile>T\<preceq>rT))"
+  (\<forall>pn\<in>set pns. map_of lvars pn = None) \<and>
+  (\<forall>(vn,T)\<in>set lvars. is_type G T) &
+  (let E = (G,map_of lvars(pns[\<mapsto>]pTs)(This\<mapsto>Class C)) in
+   E\<turnstile>blk\<surd> \<and> (\<exists>T. E\<turnstile>res::T \<and> G\<turnstile>T\<preceq>rT))"
 
 syntax 
  wf_java_prog :: "java_mb prog => bool"
@@ -234,7 +233,8 @@ apply ( drule field_fields)
 apply ( drule (1) fields_is_type)
 apply (  simp (no_asm_simp))
 apply  (assumption)
-apply (auto dest!: max_spec2mheads method_wf_mdecl is_type_rTI simp add: wf_mdecl_def)
+apply (auto dest!: max_spec2mheads method_wf_mdecl is_type_rTI 
+            simp add: wf_mdecl_def)
 done
 
 lemmas ty_expr_is_type = wt_is_type [THEN conjunct1,THEN mp, COMP swap_prems_rl]
