src/HOL/MicroJava/J/Eval.thy
@@ -4,7 +4,7 @@
     Copyright   1999 Technische Universitaet Muenchen
 *)
 
-header "Operational Evaluation (big-step) Semantics"
+header "Operational Evaluation (big step) Semantics"
 
 theory Eval = State + WellType:
 
@@ -40,24 +40,24 @@ translations
   "G\<turnstile>s -c    -> (x,s')" <= "(s, c, x, s') \<in> exec G"
   "G\<turnstile>s -c    ->    s' " == "(s, c,    s') \<in> exec G"
 
+
 inductive "eval G" "evals G" "exec G" intros
 
-(* evaluation of expressions *)
+  (* evaluation of expressions *)
 
-  (* cf. 15.5 *)
-  XcptE:"G\<turnstile>(Some xc,s) -e\<succ>arbitrary-> (Some xc,s)"
+  XcptE:"G\<turnstile>(Some xc,s) -e\<succ>arbitrary-> (Some xc,s)"  -- "cf. 15.5"
 
-  (* cf. 15.8.1 *)
+  -- "cf. 15.8.1"
   NewC: "[| h = heap s; (a,x) = new_Addr h;
             h'= h(a\<mapsto>(C,init_vars (fields (G,C)))) |] ==>
          G\<turnstile>Norm s -NewC C\<succ>Addr a-> c_hupd h' (x,s)"
 
-  (* cf. 15.15 *)
+  -- "cf. 15.15"
   Cast: "[| G\<turnstile>Norm s0 -e\<succ>v-> (x1,s1);
             x2 = raise_if (\<not> cast_ok G C (heap s1) v) ClassCast x1 |] ==>
          G\<turnstile>Norm s0 -Cast C e\<succ>v-> (x2,s1)"
 
-  (* cf. 15.7.1 *)
+  -- "cf. 15.7.1"
   Lit:  "G\<turnstile>Norm s -Lit v\<succ>v-> Norm s"
 
   BinOp:"[| G\<turnstile>Norm s -e1\<succ>v1-> s1;
@@ -66,29 +66,27 @@ inductive "eval G" "evals G" "exec G" intros
                            | Add => Intg (the_Intg v1 + the_Intg v2)) |] ==>
          G\<turnstile>Norm s -BinOp bop e1 e2\<succ>v-> s2"
 
-  (* cf. 15.13.1, 15.2 *)
+  -- "cf. 15.13.1, 15.2"
   LAcc: "G\<turnstile>Norm s -LAcc v\<succ>the (locals s v)-> Norm s"
 
-  (* cf. 15.25.1 *)
+  -- "cf. 15.25.1"
   LAss: "[| G\<turnstile>Norm s -e\<succ>v-> (x,(h,l));
             l' = (if x = None then l(va\<mapsto>v) else l) |] ==>
          G\<turnstile>Norm s -va::=e\<succ>v-> (x,(h,l'))"
 
-
-  (* cf. 15.10.1, 15.2 *)
+  -- "cf. 15.10.1, 15.2"
   FAcc: "[| G\<turnstile>Norm s0 -e\<succ>a'-> (x1,s1); 
             v = the (snd (the (heap s1 (the_Addr a'))) (fn,T)) |] ==>
          G\<turnstile>Norm s0 -{T}e..fn\<succ>v-> (np a' x1,s1)"
 
-  (* cf. 15.25.1 *)
+  -- "cf. 15.25.1"
   FAss: "[| G\<turnstile>     Norm s0  -e1\<succ>a'-> (x1,s1); a = the_Addr a';
             G\<turnstile>(np a' x1,s1) -e2\<succ>v -> (x2,s2);
             h  = heap s2; (c,fs) = the (h a);
             h' = h(a\<mapsto>(c,(fs((fn,T)\<mapsto>v)))) |] ==>
          G\<turnstile>Norm s0 -{T}e1..fn:=e2\<succ>v-> c_hupd h' (x2,s2)"
 
-
-  (* cf. 15.11.4.1, 15.11.4.2, 15.11.4.4, 15.11.4.5, 14.15 *)
+  -- "cf. 15.11.4.1, 15.11.4.2, 15.11.4.4, 15.11.4.5, 14.15"
   Call: "[| G\<turnstile>Norm s0 -e\<succ>a'-> s1; a = the_Addr a';
             G\<turnstile>s1 -ps[\<succ>]pvs-> (x,(h,l)); dynT = fst (the (h a));
             (md,rT,pns,lvars,blk,res) = the (method (G,dynT) (mn,pTs));
@@ -96,47 +94,50 @@ inductive "eval G" "evals G" "exec G" intros
             G\<turnstile> s3 -res\<succ>v -> (x4,s4) |] ==>
          G\<turnstile>Norm s0 -{C}e..mn({pTs}ps)\<succ>v-> (x4,(heap s4,l))"
 
-(* evaluation of expression lists *)
 
-  (* cf. 15.5 *)
+  -- "evaluation of expression lists"
+
+  -- "cf. 15.5"
   XcptEs:"G\<turnstile>(Some xc,s) -e[\<succ>]arbitrary-> (Some xc,s)"
 
-  (* cf. 15.11.??? *)
+  -- "cf. 15.11.???"
   Nil:  "G\<turnstile>Norm s0 -[][\<succ>][]-> Norm s0"
 
-  (* cf. 15.6.4 *)
+  -- "cf. 15.6.4"
   Cons: "[| G\<turnstile>Norm s0 -e  \<succ> v -> s1;
             G\<turnstile>     s1 -es[\<succ>]vs-> s2 |] ==>
          G\<turnstile>Norm s0 -e#es[\<succ>]v#vs-> s2"
 
-(* execution of statements *)
 
-  (* cf. 14.1 *)
+  -- "execution of statements"
+
+  -- "cf. 14.1"
   XcptS:"G\<turnstile>(Some xc,s) -c-> (Some xc,s)"
 
-  (* cf. 14.5 *)
+  -- "cf. 14.5"
   Skip: "G\<turnstile>Norm s -Skip-> Norm s"
 
-  (* cf. 14.7 *)
+  -- "cf. 14.7"
   Expr: "[| G\<turnstile>Norm s0 -e\<succ>v-> s1 |] ==>
          G\<turnstile>Norm s0 -Expr e-> s1"
 
-  (* cf. 14.2 *)
+  -- "cf. 14.2"
   Comp: "[| G\<turnstile>Norm s0 -c1-> s1;
             G\<turnstile>     s1 -c2-> s2|] ==>
          G\<turnstile>Norm s0 -c1;; c2-> s2"
 
-  (* cf. 14.8.2 *)
+  -- "cf. 14.8.2"
   Cond: "[| G\<turnstile>Norm s0  -e\<succ>v-> s1;
             G\<turnstile> s1 -(if the_Bool v then c1 else c2)-> s2|] ==>
          G\<turnstile>Norm s0 -If(e) c1 Else c2-> s2"
 
-  (* cf. 14.10, 14.10.1 *)
+  -- "cf. 14.10, 14.10.1"
   LoopF:"[| G\<turnstile>Norm s0 -e\<succ>v-> s1; \<not>the_Bool v |] ==>
          G\<turnstile>Norm s0 -While(e) c-> s1"
   LoopT:"[| G\<turnstile>Norm s0 -e\<succ>v-> s1;  the_Bool v;
-	    G\<turnstile>s1 -c-> s2; G\<turnstile>s2 -While(e) c-> s3 |] ==>
+      G\<turnstile>s1 -c-> s2; G\<turnstile>s2 -While(e) c-> s3 |] ==>
          G\<turnstile>Norm s0 -While(e) c-> s3"
+
 
 lemmas eval_evals_exec_induct = eval_evals_exec.induct [split_format (complete)]
 
