src/HOL/MicroJava/J/State.thy
@@ -8,58 +8,57 @@ header "Program State"
 
 theory State = TypeRel + Value:
 
-types	fields_
-	= "(vname \<times> cname \<leadsto> val)" (* field name, defining class, value *)
+types 
+  fields_ = "(vname \<times> cname \<leadsto> val)"  -- "field name, defining class, value"
 
-        obj = "cname \<times> fields_"	(* class instance with class name and fields *)
+  obj = "cname \<times> fields_"    -- "class instance with class name and fields"
 
 constdefs
-  obj_ty	:: "obj => ty"
+  obj_ty  :: "obj => ty"
  "obj_ty obj  == Class (fst obj)"
 
-  init_vars	:: "('a \<times> ty) list => ('a \<leadsto> val)"
- "init_vars	== map_of o map (\<lambda>(n,T). (n,default_val T))"
+  init_vars :: "('a \<times> ty) list => ('a \<leadsto> val)"
+ "init_vars == map_of o map (\<lambda>(n,T). (n,default_val T))"
   
-datatype xcpt		(* exceptions *)
-	= NullPointer
-	| ClassCast
-	| OutOfMemory
 
-types	aheap  = "loc \<leadsto> obj" (** "heap" used in a translation below **)
-        locals = "vname \<leadsto> val"	
+types aheap  = "loc \<leadsto> obj"    -- {* "@{text heap}" used in a translation below *}
+      locals = "vname \<leadsto> val"  -- "simple state, i.e. variable contents"
 
-        state		(* simple state, i.e. variable contents *)
-	= "aheap \<times> locals"
-	(* heap, local parameter including This *)
+      state  = "aheap \<times> locals"      -- "heap, local parameter including This"
+      xstate = "xcpt option \<times> state" -- "state including exception information"
 
-	xstate		(* state including exception information *)
-	 = "xcpt option \<times> state"
+
+text {*
+  System exceptions are allocated in all heaps, 
+  and they don't carry any information other than their type: *}
+axioms
+  system_xcpt_allocated: "(hp::aheap) (XcptRef x) = Some (Xcpt x, empty)"
+
 
 syntax
-  heap		:: "state => aheap"
-  locals	:: "state => locals"
-  Norm		:: "state => xstate"
+  heap    :: "state => aheap"
+  locals  :: "state => locals"
+  Norm    :: "state => xstate"
 
 translations
   "heap"   => "fst"
   "locals" => "snd"
-  "Norm s" == "(None,s)"  
+  "Norm s" == "(None,s)"
 
 constdefs
-
-  new_Addr	:: "aheap => loc \<times> xcpt option"
+  new_Addr  :: "aheap => loc \<times> xcpt option"
  "new_Addr h == SOME (a,x). (h a = None \<and>  x = None) |  x = Some OutOfMemory"
 
-  raise_if	:: "bool => xcpt => xcpt option => xcpt option"
+  raise_if  :: "bool => xcpt => xcpt option => xcpt option"
  "raise_if c x xo == if c \<and>  (xo = None) then Some x else xo"
 
-  np		:: "val => xcpt option => xcpt option"
+  np    :: "val => xcpt option => xcpt option"
  "np v == raise_if (v = Null) NullPointer"
 
-  c_hupd	:: "aheap => xstate => xstate"
+  c_hupd  :: "aheap => xstate => xstate"
  "c_hupd h'== \<lambda>(xo,(h,l)). if xo = None then (None,(h',l)) else (xo,(h,l))"
 
-  cast_ok	:: "'c prog => cname => aheap => val => bool"
+  cast_ok :: "'c prog => cname => aheap => val => bool"
  "cast_ok G C h v == v = Null \<or> G\<turnstile>obj_ty (the (h (the_Addr v)))\<preceq> Class C"
 
 lemma obj_ty_def2 [simp]: "obj_ty (C,fs) = Class C"
@@ -93,7 +92,8 @@ apply (unfold raise_if_def)
 apply auto
 done
 
-lemma raise_if_Some2 [simp]: "raise_if c z (if x = None then Some y else x) \<noteq> None"
+lemma raise_if_Some2 [simp]: 
+  "raise_if c z (if x = None then Some y else x) \<noteq> None"
 apply (unfold raise_if_def)
 apply(induct_tac "x")
 apply auto
@@ -105,12 +105,14 @@ apply (unfold raise_if_def)
 apply auto
 done
 
-lemma raise_if_NoneD [rule_format (no_asm)]: "raise_if c x y = None --> \<not> c \<and>  y = None"
+lemma raise_if_NoneD [rule_format (no_asm)]: 
+  "raise_if c x y = None --> \<not> c \<and>  y = None"
 apply (unfold raise_if_def)
 apply auto
 done
 
-lemma np_NoneD [rule_format (no_asm)]: "np a' x' = None --> x' = None \<and>  a' \<noteq> Null"
+lemma np_NoneD [rule_format (no_asm)]: 
+  "np a' x' = None --> x' = None \<and>  a' \<noteq> Null"
 apply (unfold np_def raise_if_def)
 apply auto
 done
